tests/BoogieInd.v
@@ -1,0 +1,416 @@
+
+
+Require Import Coq.ZArith.BinInt.
+Require Import Coq.Classes.EquivDec.
+
+Section Boogie.
+
+  Inductive Typ := 
+  | TInt.
+
+  Scheme Equality for Typ.
+
+  Variable (Var: Typ -> Set).
+  Variable (var_eq_dec : forall t, EqDec (Var t) eq).
+
+  Inductive Expr : Typ -> Type := 
+  | Plus : Expr TInt -> Expr TInt -> Expr TInt
+  | Minus : Expr TInt -> Expr TInt -> Expr TInt
+  | ILit : Z -> Expr TInt
+  | EVar : forall {t}, Var t -> Expr t.
+
+  Definition Value (t: Typ) := 
+    match t with 
+    | TInt => Z
+    end.
+
+  Definition State := forall t (v: Var t), Value t.
+
+  Definition put {t} (v: Var t) (rhs: Value t) (st: State) : State := 
+    fun t' (v': Var t') =>
+      match Typ_eq_dec t t' with 
+      | left H => 
+        if v' == (eq_rect _ _ v _ H) then (eq_rect _ _ rhs _ H) else st _ v'
+      | right _ => st _ v'
+      end.
+
+  Definition get {t} (v: Var t) (st: State) : Value t := st _ v.
+
+  Fixpoint eval_expr {t} (st: State) (e: Expr t) : Value t.
+  refine (
+    match e in Expr t' return Value t' with 
+    | Plus l r => (eval_expr _ st l + eval_expr _ st r)%Z
+    | Minus l r => (eval_expr _ st l - eval_expr _ st r)%Z
+    | ILit v => v
+    | EVar v => get v st
+    end
+  ).
+  Defined.
+
+  Inductive Command := 
+  | Seq: forall (c1 c2 : Command), Command
+  | Assign: forall {t} (v: Var t) (rhs: Expr t), Command
+  | Assert: forall (test: State -> Prop), Command
+  | Assume: forall (test: State -> Prop), Command
+  | Havoc: forall {t} (v: Var t), Command
+  | Cond: forall (test: State -> Prop) (c_true : Command) (c_false: Command), Command.
+
+  Fixpoint semantics (c: Command) : State -> State -> Prop.
+  refine (
+    match c with 
+    | Seq c1 c2 => fun s_pre s_post => 
+      exists s', semantics c1 s_pre s' /\ semantics c2 s' s_post
+    | Assign v rhs => fun s_pre s_post => 
+      s_post = put v (eval_expr s_pre rhs) s_pre
+    | Assert test => fun s_pre s_post => test s_pre /\ s_pre = s_post
+    | Assume test => fun s_pre s_post => test s_pre /\ s_pre = s_post
+    | @Havoc t v => fun s_pre s_post => forall (rhs: Value t), s_post = put v rhs s_pre
+    | Cond test ct cf => fun s_pre s_post => 
+      (test s_pre -> semantics ct s_pre s_post) /\ (~ test s_pre -> semantics cf s_pre s_post)
+    end
+  ).
+  Defined.
+
+
+  Fixpoint wp_command (c: Command) (Pred: State -> Prop) {struct c} : State -> Prop.
+  refine (
+    match c with 
+    | Seq c1 c2 => wp_command c1 (wp_command c2 Pred)
+    | Assign v rhs => fun s => Pred (put v (eval_expr s rhs) s)
+    | Assert test => fun s => test s /\ Pred s
+    | Assume test => fun s => (test s -> Pred s)
+    | @Havoc t v => fun s => forall (rhs: Value t), Pred (put v rhs s)
+    | Cond test ct cf => fun s => (test s /\ wp_command ct Pred s) \/ (~ test s /\ wp_command cf Pred s)
+    end
+  ).
+  Defined.
+
+  (* we need inhabitance for the soundness of the Havoc rule,
+     to connect the two different versions of Havoc
+  *)
+  Definition inhabited_Typ (t: Typ) : inhabited (Value t) := 
+    match t with 
+    | TInt => inhabits 0%Z
+    end.
+
+  Lemma wp_spec :
+    forall (c: Command) (Pred: State -> Prop) (s s' : State), 
+      semantics c s s' -> 
+      wp_command c Pred s -> 
+      Pred s'.
+  Proof.
+    induction c; simpl; intros; try subst; trivial.
+    - simpl in *.
+      destruct H as [? [? ?]].
+      pose proof (IHc1 (wp_command c2 Pred)).
+      eapply IHc2.
+      * eapply H1.
+      * eapply H2; intuition eauto.
+    - intuition eauto.
+      subst; trivial.
+    - intuition eauto.
+      subst.
+      trivial.
+    - pose proof (inhabited_Typ t).
+      destruct H1 as [rhs].
+      specialize (H rhs).
+      erewrite H.
+      eapply H0.
+    - intuition eauto.
+      * eapply IHc1;
+        intuition eauto.
+      * eapply IHc2; intuition eauto.
+  Qed.
+
+  Definition pred_top := fun (s : State) => True.
+End Boogie.
+
+Section McCarthy91.
+
+  (* procedure F(n: int) returns (r: int)
+  ensures 100 < n ==> r == n - 10;
+  ensures n <= 100 ==> r == 91;
+  {
+    if (100 < n) {
+      r := n - 10;
+    } else {
+      call r := F(n + 11);
+      call r := F(r);
+    }
+  } *)
+
+  Inductive M91Vars : Typ -> Set := | R : M91Vars TInt | N : M91Vars TInt.
+
+  Definition v0_eq_dec : EqDec (M91Vars TInt) eq.
+  refine (
+    fun l => 
+      match l with 
+      | R => fun r => 
+        match r with 
+        | R => left _
+        | N => right _ 
+        end
+      | N => fun r => 
+        match r with 
+        | R => right _ 
+        | N => left _
+        end
+      end
+  ); congruence.
+  Defined.
+
+  Definition var_eq_dec (t: Typ) : EqDec (M91Vars t) eq.
+  refine (
+    fun x y => _
+  );
+  destruct t; 
+  match goal with 
+  (* | H : M91Vars TBool |- _ => inversion H
+  | H : M91Vars (TMap _ _) |- _ => inversion H *)
+  | _ => eapply v0_eq_dec
+  end.
+  Defined.
+
+  Notation assert := (@Assert M91Vars).
+  Notation assume := (@Assume M91Vars).
+  Notation seq := (@Seq M91Vars).
+  Notation top := (@pred_top M91Vars).
+
+  Notation lit := (@ILit M91Vars).
+  Notation var := (@EVar M91Vars). 
+  Notation plus := (@Plus M91Vars).
+  Notation minus := (@Minus M91Vars).
+  Notation havoc := (@Havoc M91Vars).
+
+  Infix ";;" := (seq) (at level 150).
+  Notation "x '<-' v" := (@Assign M91Vars _ x v) (at level 98).
+
+  Notation "'If' c 'Then' ct 'Else' cf" := (@Cond M91Vars c ct cf) (at level 99).
+
+  Require Import Coq.micromega.Lia.
+
+  Definition test_1 := 
+    assume (fun st => st _ R = st _ N)%Z ;;
+    R <- (plus (var R) (lit 1%Z)) ;;
+    R <- (plus (var R) (lit 1%Z)).
+
+  Goal forall st st', 
+    semantics M91Vars var_eq_dec test_1 st st' -> 
+    (st' _ N = st _ N) /\ (st' _ R = st _ N + 2)%Z.
+  Proof.
+    intros.
+    unfold semantics, test_1 in H.
+    repeat match goal with 
+    | H: ex _ |- _ => destruct H
+    | H: _ /\ _ |- _ => destruct H
+    end.
+    subst.
+    intuition.
+    simpl.
+    unfold put, get.
+    simpl.
+    erewrite H.
+    Lia.lia.
+  Qed.
+
+  Goal forall st, wp_command M91Vars var_eq_dec test_1 top st.
+  Proof.
+    intros.
+    simpl wp_command.
+    intuition.
+    exact I.
+  Qed.
+(* 
+  procedure ok2()
+{
+  var x:int, y:int;
+  var a:t1, b:t1, c:t1;
+
+  c := if x > y then a else b;
+  assert c == a || c == b;
+  assume x > y;
+  assert c == a;
+} *)
+
+  Definition test_2 := 
+    If (fun st => st _ R < st _ N)%Z
+    Then (R <- lit 10)%Z
+    Else (assert top).
+
+  Definition test_2_post_weak (s: State M91Vars) := 
+    (s _ R < s _ N -> s _ R = 10)%Z.
+  Definition test_2_post_strong (s: State M91Vars) := 
+    s _ R = 10%Z.
+
+
+  Goal forall st, wp_command M91Vars var_eq_dec test_2 test_2_post_weak st.
+  Proof.
+    intros.
+    simpl wp_command.
+    unfold put, test_2_post_weak.
+    simpl.
+    intuition.
+    assert (st _ R < st _ N \/ ~ (st _ R < st _ N))%Z by Lia.lia.
+    destruct H.
+    - left; intuition.
+    - right; intuition; exact I.
+  Qed.
+
+
+  Definition mc_post (st: State M91Vars) : Prop := 
+    (* ensures 100 < n ==> r == n - 10;
+       ensures n <= 100 ==> r == 91 *)
+    (((100 < st _ N) -> (st _ R = st _ N - 10)) /\ 
+    ((st _ N <= 100) -> (st _ R = 91)))%Z.
+
+  Definition mccarthy := 
+    If (fun st => 100 < st _ N)%Z
+    Then (R <- minus (var N) (lit 10))%Z
+    Else (
+      (*  call r := F(n + 11);
+          call r := F(r); *)
+      havoc R ;; 
+      havoc N ;;
+      assume mc_post
+    ).
+
+  Require Import Coq.ZArith.BinInt.
+
+  Require Import MirrorSolve.FirstOrder.
+
+  Require Import MirrorSolve.Z.
+  Require Import MirrorSolve.SMT.
+
+  Require Import MirrorSolve.HLists.
+  Require Import Coq.Lists.List.
+
+  Import HListNotations.
+  Import ListNotations.
+
+  Require Import Coq.Strings.String.
+
+  Require Import MirrorSolve.Reflection.Core.
+  Require Import MirrorSolve.Reflection.FM.
+
+  Require Import Coq.Bool.Bool.
+
+  Require Import MirrorSolve.Reflection.Tactics.
+
+  MetaCoq Quote Definition c_lt := Z.ltb.
+  MetaCoq Quote Definition c_le := Z.leb.
+  MetaCoq Quote Definition c_minus := Z.sub.
+
+  MetaCoq Quote Definition c_tru := true.
+  MetaCoq Quote Definition c_fls := false.
+
+  Notation tlit := (@tacLit sig fm_model).
+  Notation tfun := (@tacFun sig _).
+
+  Definition eq_t (t: term) (t': term) : bool := 
+    eq_term t t'.
+
+  Definition is_bool_t (t: term) : bool := 
+    orb (eq_term t c_tru) (eq_term t c_fls).
+
+
+  MetaCoq Quote Definition c_zpos := Zpos.
+  MetaCoq Quote Definition c_zneg := Zneg.
+  MetaCoq Quote Definition c_z0 := Z0.
+
+  Definition is_z_t (t: term) : bool :=
+    match t with 
+    | tApp t' _ => 
+      orb (eq_term t' c_zpos) (eq_term t' c_zneg)
+    | _ => eq_term t c_z0
+    end.
+
+  Program Definition match_tacs : list ((term -> bool) * tac_syn sig fm_model) := [
+        (eq_t c_lt, tfun {| deep_f := Lt |})
+      ; (eq_t c_le,  tfun {| deep_f := Lte |})
+      ; (eq_t c_minus, tfun {| deep_f := Sub |})
+      ; (is_bool_t, tlit bool_lit (fun b => existT _ BS b) (fun b _ => existT _ BS (TFun _ (BLit b) hnil)))
+      ; (is_z_t, tlit z_lit (fun z => existT _ ZS z) (fun z _ => existT _ ZS (TFun _ (ZLit z) hnil)))
+    ]. 
+
+  MetaCoq Quote Definition bool_ind := (bool).
+  MetaCoq Quote Definition z_ind := (Z).
+
+  Definition match_inds : list (term * sorts) := [
+        (bool_ind, BS)
+      ; (z_ind, ZS)
+    ].
+
+  (* configure backend *)
+
+  Declare ML Module "mirrorsolve".
+
+  RegisterSMTSort BS SBool.
+  RegisterSMTSort ZS SInt.
+
+  RegisterSMTFun Lt "<" 2.
+  RegisterSMTFun Lte "<=" 2.
+  RegisterSMTFun Sub "-" 2.
+
+  RegisterSMTBuiltin BLit BoolLit.
+  RegisterSMTBuiltin ZLit IntLit.
+
+  Require Import MirrorSolve.Axioms.
+
+  Import UnsoundAxioms.
+
+  MetaCoq Quote Definition mccarthy_vc := (forall v : Z,
+    (100 <? v)%Z = true /\
+    ((100 <? v)%Z = true -> (v - 10)%Z = (v - 10)%Z) /\
+    ((v <=? 100)%Z = true -> (v - 10)%Z = 91%Z) \/
+    (100 <? v)%Z <> true /\
+    (forall rhs rhs0 : Z,
+    ((100 <? rhs0)%Z = true -> rhs = (rhs0 - 10)%Z) /\
+    ((rhs0 <=? 100)%Z = true -> rhs = 91%Z) ->
+    ((100 <? rhs0)%Z = true -> rhs = (rhs0 - 10)%Z) /\
+    ((rhs0 <=? 100)%Z = true -> rhs = 91%Z))).
+
+  Goal forall st st',
+    semantics M91Vars var_eq_dec mccarthy st st' -> 
+    mc_post st'.
+  Proof.
+    intros.
+    eapply wp_spec; eauto.
+    clear H.
+    simpl wp_command.
+    unfold BoogieInd.put, BoogieInd.get, mc_post.
+    simpl.
+    generalize (st _ McCarthy91.N).
+    simpl.
+    setoid_rewrite <- Z.ltb_lt.
+    setoid_rewrite <- Z.leb_le.
+    Transparent denote_tm.
+    match goal with 
+    | |- ?G => 
+      eapply denote_extract_specialized with (s := sig) (m := fm_model) (sorts_eq_dec := sorts_eq_dec) (match_tacs := match_tacs) (match_inds := match_inds) (p' := G) (t := mccarthy_vc)
+    end.
+
+    simpl_denote_tm.
+    simpl_extract_tm.
+    discharge_equiv_denote_orig; autorewrite with mod_fns in *; intuition eauto.
+    specialize (H x).
+    destruct H; [left | right]; 
+    discharge_equiv_denote_orig; autorewrite with mod_fns in *; intuition eauto.
+    
+    let v' := fresh "v" in 
+    let f' := fresh "f" in 
+    match goal with 
+    | |- interp_fm ?v ?f => 
+      set (v' := v);
+      set (f' := f)
+    end;
+    vm_compute in f';
+    subst v';
+    subst f'.
+
+    match goal with 
+    | |- ?G => check_interp_pos G; eapply interp_true
+    end.
+
+  Qed.
+
+End McCarthy91.
